

Corollary. Let $A \in F^{m \times n}$, $B \in F^{n \times p}$. Then

$$(AB)^T = B^T A^T.$$

Proof. Let $U = F^p$, $V = F^n$, $W = F^m$. Let α, β, γ be the standard ordered bases of U, V, W respectively. Let $\alpha^*, \beta^*, \gamma^*$ be the ordered bases for U^*, V^*, W^* dual to α, β, γ respectively. Let $T \in \mathcal{L}(U, V)$, $\sigma \in \mathcal{L}(V, W)$ be the linear maps with ${}_{\beta}[T]_{\alpha} = B$, ${}_{\gamma}[\sigma]_{\beta} = A$.

We know that ${}_{\gamma}[\sigma \circ T]_{\alpha} = {}_{\gamma}[\sigma]_{\beta} {}_{\beta}[T]_{\alpha} = AB$.

By the previous proposition,

$${}_{\beta^*}[\sigma^*]_{\gamma^*} = A^T, \quad {}_{\alpha^*}[T^*]_{\beta^*} = B^T, \quad {}_{\alpha^*}[(\sigma \circ T)^*]_{\gamma^*} = (AB)^T.$$

Since $(\sigma \circ T)^* = T^* \circ \sigma^*$, we have

$$(AB)^T = {}_{\alpha^*}[(\sigma \circ T)^*]_{\gamma^*} = {}_{\alpha^*}[T^* \circ \sigma^*]_{\gamma^*} = {}_{\alpha^*}[T^*]_{\beta^*} {}_{\beta^*}[\sigma^*]_{\gamma^*} = B^T A^T.$$

□

Prop Let U, V be f.d.v.s. over F . Let $n = \dim U, m = \dim V$. Let α, β be ordered bases for U, V respectively. Let α^*, β^* be the ordered bases for U^*, V^* dual to α, β respectively.

(i) Let $\theta \in V^*$. Then $[\theta]_{\beta^*} = \left({}_{1_F} [\theta]_{\beta} \right)^T$.

(ii) Let $\theta \in V^*$ and let $\sigma \in \mathcal{L}(U, V)$. Let $A = {}_{\beta} [\sigma]_{\alpha}$ and $v = {}_{1_F} [\theta]_{\beta} \in F^{1 \times m}$. Then $[\sigma^*(\theta)]_{\alpha^*} = (v \cdot A)^T$.

Proof. (i) Say $\beta = (f_1, \dots, f_m)$, $\beta^* = (\phi_1, \dots, \phi_m)$.

Suppose $\theta = \lambda_1 \phi_1 + \dots + \lambda_m \phi_m$, where $\lambda_1, \dots, \lambda_m \in F$.

This means that

$$[\theta]_{\beta^*} = \begin{bmatrix} \lambda_1 \\ \vdots \\ \lambda_m \end{bmatrix}.$$

Also, for $i = 1, \dots, m$,

$$\theta(f_i) = \langle \lambda_1 \phi_1 + \dots + \lambda_m \phi_m, f_i \rangle = \lambda_i,$$

$$\text{so } {}_{1_F} [\theta]_{\beta} = [\lambda_1 \dots \lambda_m].$$

$$\text{Hence } [\theta]_{\beta^*} = \left({}_{1_F} [\theta]_{\beta} \right)^T.$$

$$(ii) \quad [\sigma^*(\theta)]_{\alpha^*} = [\theta \circ \sigma]_{\alpha^*}$$

$$= \left({}_{1_F} [\theta \circ \sigma]_{\alpha} \right)^T \quad (\text{by part (a)})$$

$$= \left({}_{1_F} [\theta]_{\beta} \cdot {}_{\beta} [\sigma]_{\alpha} \right)^T$$

$$= (v \cdot A)^T$$

□

Rk It can be helpful to think of elements in the dual space as "row vectors" with dual maps acting on them by right matrix multiplication (i.e., we forget about the transposes above).

Lemma Let U, V, W be f.d.v.s. over F . Let $\sigma \in \mathcal{L}(U, V)$ and let $\varphi \in \mathcal{L}(U, W)$.

Then, there exists $Z \in \mathcal{L}(V, W)$ such that $Z\sigma = \varphi$ if and only if $\ker(\sigma) \subseteq \ker(\varphi)$.

$$\begin{array}{ccc} U & \xrightarrow{\sigma} & W \\ \sigma \downarrow & \nearrow Z & \\ V & & \end{array}$$

Rk In particular, taking $W = F$, we see that given $\eta \in U^*$, there exists $\theta \in V^*$ such that $\sigma^*(\theta) = \theta \circ \sigma = \eta$ if and only if $\ker(\sigma) \subseteq \ker(\eta)$, i.e.,

$$\eta \in \text{im}(\sigma^*) \iff \ker(\sigma) \subseteq \ker(\eta).$$

Prop. Let $\sigma \in \mathcal{L}(U, V)$. Then $\text{im}(\sigma^*) = \ker(\sigma)^\perp$.

Proof. Let $\eta \in U^*$. Then

$$\begin{aligned}\eta \in \text{im}(\sigma^*) &\iff \ker(\sigma) \subseteq \ker(\eta) \\ &\iff \eta(x) = 0 \quad \forall x \in \ker(\sigma) \\ &\iff \langle \eta, x \rangle = 0 \quad \forall x \in \ker(\sigma) \\ &\iff \eta \in \ker(\sigma)^\perp.\end{aligned}$$

Therefore $\text{im}(\sigma^*) = \ker(\sigma)^\perp$. □

Rk. Previously, we also proved that $\ker(\sigma^*) = \text{im}(\sigma)^\perp$.

Prop. Let $\sigma \in \mathcal{L}(U, V)$. Then:

(i) σ is injective if and only if σ^* is surjective.

(ii) σ is surjective if and only if σ^* is injective.

Proof.

$$\begin{aligned}\text{(i) } \sigma \text{ is injective} &\iff \ker(\sigma) = \{0\} \\ &\iff \ker(\sigma)^\perp = U^* \\ &\iff \text{im}(\sigma^*) = U^* \\ &\iff \sigma^* \text{ is surjective.}\end{aligned}$$

$$\begin{aligned}
 \text{(ii) } \sigma \text{ is surjective} &\iff \text{im}(\sigma) = V \\
 &\iff \text{im}(\sigma)^\perp = \{0\} \\
 &\iff \ker(\sigma^*) = \{0\} \\
 &\iff \sigma^* \text{ is injective.}
 \end{aligned}$$

Example Let U, V be \mathbb{R} -vector spaces. Suppose $\dim(U) = 3, \dim(V) = 2$.

Let $\alpha = (e_1, e_2, e_3), \beta = (f_1, f_2)$ be ordered bases for U, V , respectively. Let $\alpha^* = (\varepsilon_1, \varepsilon_2, \varepsilon_3), \beta^* = (\phi_1, \phi_2)$ be the ordered bases for U^*, V^* dual to α, β , respectively. Let $\sigma \in \mathcal{L}(U, V)$ be the linear map with ${}_{\beta}[\sigma]_{\alpha} = A = \begin{bmatrix} 1 & 2 & -2 \\ 2 & 4 & -4 \end{bmatrix}$.

$$\bullet \text{Col}(A) = \text{span} \left\{ \begin{bmatrix} 1 \\ 2 \end{bmatrix}, \begin{bmatrix} 2 \\ 4 \end{bmatrix}, \begin{bmatrix} -2 \\ -4 \end{bmatrix} \right\} = \text{span} \left\{ \begin{bmatrix} 1 \\ 2 \end{bmatrix} \right\},$$

$$\text{so } \text{im}(\sigma) = \text{span} \{ f_1 + 2f_2 \}.$$

$$\begin{aligned}
 \bullet \text{Null}(A) &= \left\{ \begin{bmatrix} x \\ y \\ z \end{bmatrix} \mid A \begin{bmatrix} x \\ y \\ z \end{bmatrix} = \begin{bmatrix} 0 \\ 0 \end{bmatrix} \right\} \\
 &= \left\{ \begin{bmatrix} x \\ y \\ z \end{bmatrix} \mid x + 2y - 2z = 0, 2x + 4y - 4z = 0 \right\} \\
 &= \text{span} \left\{ \begin{bmatrix} -2 \\ 1 \\ 0 \end{bmatrix}, \begin{bmatrix} 2 \\ 0 \\ 1 \end{bmatrix} \right\}
 \end{aligned}$$

so $\ker(\sigma) = \text{span} \{ -2e_1 + e_2, 2e_1 + e_3 \}$.

• $\text{Row}(A) = \text{span} \{ [1 \ 2 \ -2], [2 \ 4 \ -4] \} \quad \Bigg| \quad \text{Col}(A^T) = \text{span} \left\{ \begin{bmatrix} 1 \\ 2 \\ -2 \end{bmatrix} \right\}$
 $= \text{span} \{ [1 \ 2 \ -2] \},$

so $\text{im}(\sigma^*) = \text{span} \{ e_1 + 2e_2 - 2e_3 \}$

Identify $\mathbb{R}^{1 \times 3}$ with $(\mathbb{R}^{3 \times 1})^*$ by identifying each element

$[\alpha \ \beta \ \gamma] \in \mathbb{R}^{1 \times 3}$ with the linear map

$$\mathbb{R}^{3 \times 1} \longrightarrow \mathbb{R}$$

$$\begin{bmatrix} x \\ y \\ z \end{bmatrix} \longmapsto [\alpha \ \beta \ \gamma] \begin{bmatrix} x \\ y \\ z \end{bmatrix} = \alpha x + \beta y + \gamma z.$$

Similarly, identify $\mathbb{R}^{1 \times 2}$ with $(\mathbb{R}^{2 \times 1})^*$. Then:

• $\text{Null}(A)^\perp = \left\{ [\alpha \ \beta \ \gamma] \mid [\alpha \ \beta \ \gamma] \begin{bmatrix} x \\ y \\ z \end{bmatrix} = 0 \text{ for all } \begin{bmatrix} x \\ y \\ z \end{bmatrix} \in \text{Null}(A) \right\}$

$$= \left\{ [\alpha \ \beta \ \gamma] \mid [\alpha \ \beta \ \gamma] \begin{bmatrix} -2 \\ 1 \\ 0 \end{bmatrix} = [\alpha \ \beta \ \gamma] \begin{bmatrix} 2 \\ 0 \\ 1 \end{bmatrix} = 0 \right\}$$

$$= \left\{ [\alpha \ \beta \ \gamma] \mid -2\alpha + \beta = 0, 2\alpha + \gamma = 0 \right\}$$

$$= \text{span} \{ [1 \ 2 \ -2] \}.$$

Then $\ker(\sigma)^\perp = \text{span} \{ e_1 + 2e_2 - 2e_3 \}$.

Note that $\text{Row}(A) = \text{Null}(A)^\perp$, so $\text{im}(\sigma^*) = \ker(\sigma)^\perp$.

$$\begin{aligned} \bullet \text{Null}^T(A) &:= \left\{ [0 \ v] \mid [0 \ v] A = [0 \ 0 \ 0] \right\} & \text{Null}(A^T) &= \text{span} \left\{ \begin{bmatrix} 2 \\ -1 \end{bmatrix} \right\} \\ &= \text{span} \{ [2 \ -1] \} \end{aligned}$$

so $\ker(\sigma^*) = \text{span} \{ 2\phi_1 - \phi_2 \}$.

$$\begin{aligned} \bullet \text{Col}(A)^\perp &= \left\{ [0 \ v] \mid [0 \ v] \begin{bmatrix} x \\ y \end{bmatrix} \text{ for all } \begin{bmatrix} x \\ y \end{bmatrix} \in \text{Col}(A) \right\} \\ &= \left\{ [0 \ v] \mid [0 \ v] \begin{bmatrix} 1 \\ 2 \end{bmatrix} = 0 \right\} \\ &= \text{span} \{ [2 \ -1] \} \end{aligned}$$

So $\text{im}(\sigma)^\perp = \text{span} \{ 2\phi_1 - \phi_2 \}$.

Note that $\text{Null}^T(A) = \text{Col}(A)^\perp$, so $\ker(\sigma^*) = \text{im}(\sigma)^\perp$.